\documentclass{article}
\author{GONG,Xianjin}
\title{Homework 1 of Honor Calculus}

\begin{document}
\maketitle

\section{Part 1}(for peer riview)

1.1.4(9)

$
   \lim \limits_{n \to +\infty}\frac{(\sqrt[3]{n}+3)^3}{(\sqrt{n}-2)^2}
 = \lim \limits_{n \to +\infty}\frac{n+9n^\frac{2}{3} +27n^\frac{1}{3} +27}{n-4n^\frac{1}{2} +4}
 = \lim \limits_{n \to +\infty}\frac{1+9\frac{1}{n^\frac{1}{3}} +27\frac{2}{n^\frac{2}{3}} +\frac{27}{n}}
                             {1-4\frac{1}{n^\frac{1}{2}} +4\frac{1}{n}}
$

$
 =  \frac {\lim \limits_{n \to +\infty}1
            +\lim \limits_{n \to +\infty}9\frac{1}{n^\frac{1}{3}}
            +\lim \limits_{n \to +\infty}27\frac{2}{n^\frac{2}{3}}
            +\lim \limits_{n \to +\infty}\frac{27}{n}}
            {\lim \limits_{n \to +\infty}1
            -\lim \limits_{n \to +\infty}4\frac{1}{n^\frac{1}{2}}
            +\lim \limits_{n \to +\infty}4\frac{1}{n}
            }
  = \frac{1+0+0+0}{1-0-0}
  = 0
$
\\\\

1.1.6

$
When 0<p<q \ \ \ \ \lim \limits_{n \to +\infty}\frac{a_pn^p+a_p-1n^p-1+\cdots+a_1n+a_0}{b_qn^q+b_q-1n^q-1+\cdots+b_1n+b_0}
$
\end{document}
